lib/libcoq.mli
@@ -62,6 +62,8 @@ module Red_black_tree :
 
   val split : key -> 'a1 rbtree -> ('a1 rbtree * bool) * 'a1 rbtree
 
+  val union : 'a1 rbtree -> 'a1 rbtree -> 'a1 rbtree
+
   val size : 'a1 rbtree -> int
 
   val next : key -> 'a1 rbtree -> (key * 'a1) option
@@ -79,9 +81,9 @@ module Red_black_tree :
 
   val rbtree_eqb : 'a1 rbtree -> 'a1 rbtree -> bool
 
-  val union_aux : 'a1 rbtree -> (key * 'a1) list -> 'a1 rbtree
+  val slow_union_aux : 'a1 rbtree -> (key * 'a1) list -> 'a1 rbtree
 
-  val union : 'a1 rbtree -> 'a1 rbtree -> 'a1 rbtree
+  val slow_union : 'a1 rbtree -> 'a1 rbtree -> 'a1 rbtree
 
   val delete : key -> 'a1 rbtree -> 'a1 rbtree * bool
  end
